Work up to date

Main.v
@@ -5,7 +5,8 @@ Require Import List.
 Require Import EqNat.
 Require Import Dblib.DblibTactics.
 Require Import Dblib.DeBruijn.
-
+Require Import Dblib.Environments.
+Check lookup_insert_recent.
 (* Require Import DblibTactics.
 Require Import Debruijn *)
 
@@ -13,8 +14,20 @@ Notation "[ ]" := nil : list_scope.
 Notation "[ x ]" := (cons x nil) : list_scope.
 Notation "[ x ; y ; .. ; z ]" := (cons x (cons y .. (cons z nil) ..)) : list_scope.
 
-Inductive value : Type :=
-|VUnit : value | VName :> nat -> value.
+Fixpoint delete {A : Type} (x : nat) (e : env A) : env A :=
+  match x, e with
+  | _, nil => nil
+  | 0, (_ :: e) => e
+  | (S n'), (e :: es) =>  delete n' es
+  end.
+
+Fixpoint update {A : Type} (x : nat) (o : option A) (e : env A) : env A :=
+  match x, e with
+  | 0, nil => nil
+  | 0, (_ :: xs) => o :: xs
+  | S n', nil => nil
+  | S n', (x :: xs) => x :: (update n' o xs)
+  end.
 
 Inductive type : Set :=
 | TSession :> stype -> type
@@ -23,7 +36,6 @@ Inductive type : Set :=
 | T0Nul : type
 | TSum : type -> type -> type
 | TLoli : type -> type -> type
-| TSharp : stype -> type
 with stype : Set :=
 |TSendEnd : stype
 |TRecvEnd : stype
@@ -35,53 +47,12 @@ with ltype : Prop :=
 | lAllow : type -> type -> ltype.
              *)
 
-Definition env := list (option type).
-Definition emptyEnv: env := [].
-
-Fixpoint emptyEnvQ(e:env):bool :=
-  match e with
-  | [] => true
-  | (Some _ :: _) => false
-  | (None :: xs) => emptyEnvQ xs
-  end.
-
-(* Environmental sanity check *)
-Example emptyEnv1: emptyEnvQ [] = true.
-Proof. reflexivity. Qed.
-Example emptyEnv2: emptyEnvQ [Some T1Nul] = false.
-Proof. reflexivity. Qed.
-
- Fixpoint dual(s:stype):stype:=
-  match s with
-  | TSendEnd => TRecvEnd
-  |TRecvEnd => TSendEnd
-  |(TSend T s) => TRecv T (dual s)
-  |(TRecv T s) => TSend T (dual s)
-  end.
-
-(* Inductive term: env -> type -> env -> Prop :=
-| E1Nul: forall g, term g T1Nul g
-| EVar : forall g t s, t <> (TSession s) -> term g t g
-(* | EPair : forall g g' g'', term g M g -> term g' N g' -> term (res g g') (TProd M N) (res g g') *)
-| EInl : forall g t u, term g t g -> term g (TSum t u) g
-| EInr : forall g t u, term g u g -> term g (TSum t u) g.
- *)
-
- Inductive constant : Type :=
- | send : constant
- | receive : constant
- | fork : constant
- | wait : constant
- | link : constant.
-
-(* GV Constants *)
-(*Inductive constant :=
-  | send : forall S T, TLoli (TProd T (TSend T S)) S -> constant.
-Definition receive{S : stype}{T : type} := TLoli (TRecv T S) (TProd T S).
-Definition fork{S : stype} := TLoli (TLoli S TSendEnd) (dual S).
-Definition wait:= TLoli TRecvEnd T1Nul.
-Definition link{S : stype} := TLoli (TProd S (dual S)) TSendEnd.
-*)
+Inductive constant : Set :=
+| send : constant
+| receive : constant
+| fork : constant
+| wait : constant
+| link : constant.
 
 Inductive term : Set :=
 | EVar : nat -> term
@@ -89,13 +60,36 @@ Inductive term : Set :=
 | ELam : term -> term
 | EApp : term -> term -> term
 | EPair : term -> term -> term
-| ELetPair : term -> term -> term -> term
+| ELetPair : nat -> nat -> term -> term -> term
 | EInl : term -> term
 | EInr : term -> term
 | ECase : term -> term -> term -> term
 | EUnit : term
 | ELetUnit : term -> term -> term
 | EAbsurd : term -> term.
+
+Check (@lift term).
+Eval cbv in (shift 0 (ELam (EVar 0))).
+
+Notation "T * S" := (TProd T S).
+Notation "T -o U" := (TLoli T U) (at level 0, right associativity).
+Notation "! T ; S" := (TSend T S) (at level 0).
+Notation "? T ; S" := (TRecv T S) (at level 0).
+Notation "end!" := TSendEnd.
+Notation "end?" := TRecvEnd.
+
+Definition Env := env type.
+
+Fixpoint dual(s:stype):stype:=
+ match s with
+ | end! => end?
+ | end? => end!
+ | ! T; s => ? T; (dual s)
+ | ? T; s => ! T; (dual s)
+ end.
+
+Lemma dual_inverse : forall s, dual (dual s) = s.
+Proof. induction s; simpl; try rewrite IHs; try reflexivity. Qed.
 
 Instance Var_term : Var term := {
   var := EVar
@@ -108,7 +102,7 @@ Fixpoint traverse_term (f : nat -> nat -> term) l t :=
   | ELam t => ELam (traverse_term f (1+l) t)
   | EApp t1 t2 => EApp (traverse_term f l t1) (traverse_term f l t2)
   | EPair t1 t2 => EPair (traverse_term f l t1) (traverse_term f l t2)
-  | ELetPair t t2 t3 => ELetPair (traverse_term f l t) (traverse_term f l t2) (traverse_term f l t3)
+  | ELetPair v1 v2 t1 t2 => ELetPair v1 v2 (traverse_term f l t1) (traverse_term f l t2)
   | EInl t => EInl (traverse_term f l t)
   | EInr t => EInr (traverse_term f l t)
   | ECase t t1 t2 => ECase (traverse_term f l t) (traverse_term f l t1) (traverse_term f l t2)
@@ -116,6 +110,8 @@ Fixpoint traverse_term (f : nat -> nat -> term) l t :=
   | ELetUnit M N => ELetUnit (traverse_term f l M) (traverse_term f l N)
   | EAbsurd M => EAbsurd (traverse_term f l M)
   end.
+
+Notation "()" := EUnit.
 
 Instance Traverse_term : Traverse term term := {
                                                 traverse := traverse_term
@@ -136,25 +132,172 @@ Proof. constructor. prove_traverse_identifies_var. Qed.
 Instance TraverseVarIsIdentity_term : @TraverseVarIsIdentity term _ term _.
 Proof. constructor. prove_traverse_var_is_identity. Qed.
 
-(*
-Inductive type_check : env -> term -> type -> Prop :=
-  (*  | type_Val : forall t, (type_check (EVal) t). *)
-| type_var : forall (g : env)(e:term)(t:type)(s : stype), t <> (TSharp s) -> type_check g e t.
-(* | type_fun : forall (g : env)(e : term)(t:type), *)
+Inductive value : term -> Prop :=
+| VVar : forall x, value (EVar x)
+| VAbs : forall M, value (ELam M)
+| VNul : value EUnit
+| VPair : forall V W, value V -> value W -> value (EPair V W)
+| VInl : forall V, value V -> value (EInl V)
+| VInr : forall V, value V -> value (EInr V).
+
+(* 
+(* GV Constants *)
+Definition send_type{S : stype}{T : type} := ((TProd T (! T;S)) -o S).
+Definition rec_type{S : stype}{T : type} := (? T;S) -o (TProd T S).
+Definition fork_type{S : stype} := ((S -o end!) -o (dual S)).
+Definition wait_type := end? -o T1Nul.
+Definition link_type{S : stype} := (TProd S (dual S)) -o end!.
 *)
 
-Notation "! T . S" := (TSend T S) (at level 20).
-Notation "? T . S" := (TRecv T S) (at level 20).
-Notation "end!" := TSendEnd.
-Notation "end?" := TRecvEnd. 
+Fixpoint tl_error{A} (x : list A): option (list A):=
+  match x with
+  | [] => None
+  | (_ :: xs) => Some xs
+  end.
 
-Lemma dual_inverse : forall s, dual (dual s) = s.
-Proof. induction s; simpl.
-       - reflexivity.
-       - reflexivity.
-       - rewrite IHs. reflexivity.
-       - rewrite IHs. reflexivity.
+Inductive check: Env -> term -> Env -> type -> Prop :=
+| CVar : forall E x T, lookup x E = Some T ->
+                  check E (EVar x) (update x None E) T
+| CLam : forall E E' E'' M T U, check (insert 0 T E) M E' U ->
+                       tl_error E' = Some E'' ->
+                       check E (ELam M) E'' (T -o U)
+| CSend : forall E E' T S M, check E M E' (TProd T (! T; S)) ->
+                        check E (ECApp send M) E' S
+| CRecv : forall E E' T S M, check E M E' (? T;S) ->
+                        check E (ECApp receive M) E' (TProd T S)
+| CFork : forall E E' S M, check E M E' ((TSession S) -o end!) ->
+                      check E (ECApp fork M) E' (dual S)
+| CWait : forall E E' M, check E M E' end? ->
+                    check E (ECApp wait M) E' T1Nul
+| CApp : forall E E' E'' M N T U, check E M E' (T -o U) ->
+                             check E' N E'' T ->
+                             check E (EApp M N) E'' U
+| CPair: forall E E' E'' M N T U, check E M E' T ->
+                             check E' N E'' U ->
+                             check E (EPair M N) E'' (TProd T U)
+| CInl : forall E E' M T U, check E M E' T ->
+                       check E (EInl M) E' (TSum T U)
+| CInr : forall E E' M T U, check E M E' U ->
+                       check E (EInr M) E' (TSum T U)
+| CLetPair : forall E E' E'' M N T T' U x y, lookup x E = Some T ->
+                                        lookup y E = Some T' -> 
+                                        check E M E' (TProd T T') ->
+                                        check (insert 0 T (insert 0 T' E')) N E'' U ->
+                                        check E (ELetPair x y M N) E'' U
+| CCase : forall E E' E'' M N N' T T' U A, check E M E' (TSum T T') ->
+                                      check (insert 0 T E')  N  E'' U /\ tl_error E'' = Some A ->
+                                      check (insert 0 T' E') N'  E'' U /\ tl_error E'' = Some A ->
+                                      check E (ECase M N N') E'' U
+| CLetUnit: forall M N E E' E'' T, check E M E' T1Nul ->
+                              check E' N E'' T ->
+                              check E (ELetUnit M N) E'' T
+| CNul : forall E, check E EUnit E T1Nul.
+
+Hint Constructors check : check.
+
+Example check_var : check nil (ELam (EVar 0)) nil (T1Nul -o T1Nul).
+Proof. apply CLam with (E' := [None]). apply CVar. reflexivity. reflexivity. Qed.
+
+Example check_lam_pair : forall A B, check nil (ELam (ELam (EPair (EVar 1) (EVar 0)))) nil (A -o B -o (TProd A B)).
+Proof. intros.
+       apply CLam with (E' := [None]); try reflexivity.
+       apply CLam with (E' := [None; None]); try reflexivity.
+       apply CPair with (E' := [Some B; None]).
+       apply CVar. reflexivity.
+       apply CVar. reflexivity.
 Qed.
+
+Lemma lift_EVar: forall w k x, lift w k (EVar x) = EVar (lift w k x).
+Proof. intros. simpl_lift_goal. reflexivity. Qed.
+
+Lemma subst_EVar: forall v k x, subst v k (EVar x) = subst_idx v k x.
+Proof. intros. simpl_subst_goal. reflexivity. Qed.
+
+Inductive red : term -> term -> Prop :=
+| RUnit : forall M, red (ELetUnit () M) M
+| RBeta : forall M V, value V ->
+                 red (EApp (ELam M) V) (subst V 0 M)
+| RLetSub : forall x y V V' M, value V ->
+                          value V' ->
+                          red (ELetPair x y (EPair V V') M) (subst V x (subst V' y M))
+| RCApp: forall K M M', red M M' ->
+                   red (ECApp K M) (ECApp K M')
+| RVapp: forall V M M', value V ->
+                   red M M' ->
+                   red (EApp V M) (EApp V M')
+| RLetUnit : forall M M' N, red M M' ->
+                       red (ELetUnit M N) (ELetUnit M' N)
+| RPair : forall M M' N, red M M' ->
+                    red (EPair M N) (EPair M' N)
+| RVPair : forall V M M', value V ->
+                     red M M' ->
+                     red (EPair V M) (EPair V M')
+| RAbs : forall M M', red M M' ->
+                 red (ELam M) (ELam M')
+| RLetPair : forall x y M M' T, red M M' ->
+                           red (ELetPair x y T M) (ELetPair x y T M')
+| RInl : forall M M', red M M' ->
+                 red (EInl M) (EInl M')
+| RInr : forall M M', red M M' ->
+                 red (EInr M) (EInr M')
+| RCase : forall M M' N N', red M M' ->
+                       red (ECase M N N') (ECase M' N N')
+| RLeft : forall N N' V, value V ->
+                    red (ECase (EInl V) N N') (subst V 0 N)
+| RRight : forall N N' V, value V ->
+                     red (ECase (EInr V) N N') (subst V 0 N').
+
+Lemma unique: forall E E' M T U, check E M E' T -> check E M E' U -> T = U.
+Proof. intros. induction H; simpl. inversion H0; subst. 
+Abort.
+
+(* Lemma substitution:
+  forall E x t2 T1 T2,
+  j (insert x T1 E) t2 T2 ->
+  forall t1,
+  j E t1 T1 ->
+  j E (subst t1 x t2) T2.
+ *)
+
+Lemma substitution:
+  forall (E: env type) (x : nat) (t2 : term) (T1 T2 : type),
+    check (insert x T1 E) t2 (update x None E) T2 ->
+    forall (t1  : term ), value t1 ->
+          check E t1 (insert x T1 E) T1 ->
+          check (insert x T1 E) (subst t1 x t2) (update x None E) T2.
+Proof. intros.
+       induction H; simpl_subst_goal;
+         try solve [ econstructor; eauto; simpl].
+       unfold subst_idx; dblib_by_cases; simpl. apply CVar; assumption.
+       apply agree_below with (e2:= (update x0 None E0)) (k := x0)in H.
+
+       Abort.
+
+Theorem check_reduce : forall M M' E E' T, check E M E' T -> red M M' -> check E M' E' T.
+Proof. induction M; intros.
+       - inversion H0.
+       - inversion H0; subst. inversion H; subst.
+         * apply CSend with (T := T0). apply IHM; assumption.
+         * apply CRecv. apply IHM; assumption.
+         * apply CFork. apply IHM; assumption.
+         * apply CWait. apply IHM; assumption.
+       - inversion H0; inversion H; subst. apply IHM with (M' := M'0) in H5; try assumption.
+         apply CLam with (E' := E'0); assumption.
+       - inversion H; inversion H0; subst. 
+         * inversion H11; subst. 
+
+         * apply IHM2 with (M' := M'0) in H7; try assumption.
+           apply CApp with (E' := E'0)(T := T0); assumption.
+         destruct M'. inversion H0; subst. inversion H; inversion H0; subst.
+      
+(*
+         Focus 2. apply CApp with (E' := E') (T := T).
+         apply IHM1 with (M' := ) in H4
+         apply IHM2 with (M' := ) in H7.
+*)
+
+
+
 
 (*  *)
 
